ulib/FStar.BV.fsti
@@ -142,7 +142,7 @@ val int2bv_shl:
 
 val bvshl_unsafe (#n: pos) (a b : bv_t n) : Tot (bv_t n)
 
-(** Bitwise shift right *)
+(** Bitwise shift (logical) right *)
 val bvshr (#n: pos) (a: bv_t n) (s: nat) : Tot (bv_t n)
 
 val bvshr_unsafe (#n: pos) (a b : bv_t n) : Tot (bv_t n)
@@ -160,6 +160,25 @@ val int2bv_shr:
     #z: bv_t n ->
     squash (bvshr #n (int2bv #n x) y == z)
   -> Lemma (int2bv #n (shift_right #n x y) == z)
+
+(** Bitwise shift (arithmetic) right *)
+val bvashr (#n: pos) (a: bv_t n) (s: nat) : Tot (bv_t n)
+
+val bvashr_unsafe (#n: pos) (a b : bv_t n) : Tot (bv_t n)
+
+val bvashr_unsafe_sound :
+    #n: pos ->
+    #a : bv_t n ->
+    #b : bv_t n
+  -> Lemma (bvashr_unsafe #n a b = bvashr #n a (bv2int #n b))
+
+val int2bv_ashr:
+    #n: pos ->
+    #x: uint_t n ->
+    #y: uint_t n ->
+    #z: bv_t n ->
+    squash (bvashr #n (int2bv #n x) y == z)
+  -> Lemma (int2bv #n (shift_arithmetic_right #n x y) == z)
 
 (**** Arithmetic operations *)
 unfold
